

Homework 8

Jiasong Zhu

November 19, 2025

Problem 1

Solution. (i) Use coordinates $u = (u^1, \dots, u^n)$ on U and the parametrization

$$X(u) = (u^1, \dots, u^n, f(u)).$$

Then the coordinate tangent vectors are

$$X_i := \frac{\partial X}{\partial u^i} = e_i + f_i e_{n+1}, \quad f_i := \frac{\partial f}{\partial u^i}.$$

The induced metric is

$$g_{ij} = \langle X_i, X_j \rangle = \delta_{ij} + f_i f_j.$$

A normal vector is $(-f_1, \dots, -f_n, 1)$, whose length is

$$W := \sqrt{1 + \sum_{k=1}^n f_k^2}.$$

So the upward unit normal is

$$N = \frac{1}{W}(-f_1, \dots, -f_n, 1).$$

The second fundamental form is, by Lee, Prop. 8.23

$$h(X_i, X_j) = \left\langle \frac{\partial^2 X}{\partial u^i \partial u^j}, N \right\rangle.$$

We have

$$\frac{\partial^2 X}{\partial u^i \partial u^j} = f_{ij} e_{n+1}, \quad f_{ij} := \frac{\partial^2 f}{\partial u^i \partial u^j},$$

so

$$h_{ij} := h(X_i, X_j) = \langle f_{ij} e_{n+1}, N \rangle = f_{ij} N_{n+1} = \frac{f_{ij}}{W}.$$

By def of the shape operator s ,

$$\langle sX_i, X_j \rangle = h(X_i, X_j),$$

so if $s(X_j) = s^k_j X_k$, then

$$h_{ij} = g_{ik} s^k_j.$$

Thus, the components of the shape operator in graph coordinates are

$$s^k{}_j = g^{ki} h_{ij} = \frac{1}{W} g^{ki} f_{ij},$$

where (g^{ij}) is the inverse matrix of $(g_{ij}) = (\delta_{ij} + f_i f_j)$.

(ii) Now let

$$f(x) = |x|^2 = \sum_{i=1}^n (x^i)^2.$$

Then

$$f_i = \frac{\partial f}{\partial x^i} = 2x^i, \quad f_{ij} = \frac{\partial^2 f}{\partial x^i \partial x^j} = 2\delta_{ij}.$$

Hence

$$|\nabla f|^2 = \sum_i f_i^2 = 4|x|^2 = 4r^2, \quad r := |x|, \quad W = \sqrt{1 + 4r^2}.$$

From (i),

$$h_{ij} = \frac{f_{ij}}{W} = \frac{2}{W} \delta_{ij}.$$

The metric in these coordinates is

$$g_{ij} = \delta_{ij} + f_i f_j = \delta_{ij} + 4x^i x^j,$$

which is of the matrix

$$G = I + 4xx^T.$$

To find principal curvatures, we should find the eigenvalues of s , which is of the matrix

$$S = (s^i{}_j) = G^{-1}H, \quad H = (h_{ij}) = \frac{2}{W}I.$$

So $S = \frac{2}{W}G^{-1}$, and its eigenvalues are $\frac{2}{W}$ times the eigenvalues of G^{-1} .

Choose an orthonormal basis in \mathbb{R}^n so that

$$e_1 = \frac{x}{r}, \quad e_2, \dots, e_n \perp x.$$

Then

$$Ge_1 = (1 + 4r^2)e_1, \quad Ge_\alpha = e_\alpha \quad (\alpha = 2, \dots, n).$$

So the eigenvalues of G are $1 + 4r^2$ and 1. Thus the eigenvalues of G^{-1} are

$$\frac{1}{1 + 4r^2}, \quad 1.$$

Therefore the principal curvatures at a point with $|x| = r > 0$ are

$$\kappa_{\text{rad}}(r) = \frac{2}{W} \cdot \frac{1}{1 + 4r^2} = \frac{2}{(1 + 4r^2)^{3/2}},$$

in the direction of ∇f , and

$$\kappa_{\text{tan}}(r) = \frac{2}{W} = \frac{2}{\sqrt{1 + 4r^2}}$$

in each of the $n - 1$ directions orthogonal to ∇f .

At the vertex $x = 0$, we have $r = 0$, so $G(0) = I$, $h_{ij}(0) = 2\delta_{ij}$, hence

$$S(0) = 2I,$$

and all principal curvatures at $x = 0$ are

$$\kappa_1(0) = \cdots = \kappa_n(0) = 2.$$

□

Problem 2

Proof. (i) Compute first derivatives:

$$X_t = (a' \cos \theta, a' \sin \theta, b'), \quad X_\theta = (-a \sin \theta, a \cos \theta, 0).$$

$$E = \langle X_t, X_t \rangle = (a')^2 + (b')^2 = 1,$$

$$F = \langle X_t, X_\theta \rangle = 0,$$

$$G = \langle X_\theta, X_\theta \rangle = a^2.$$

So in the basis $\{X_t, X_\theta\}$,

$$g = \begin{pmatrix} 1 & 0 \\ 0 & a^2 \end{pmatrix},$$

and the coordinate lines $t = \text{const}$ (meridians) and $\theta = \text{const}$ (parallels) are orthogonal.

Compute

$$X_t \times X_\theta = (-ab' \cos \theta, -ab' \sin \theta, aa'),$$

whose length is $|X_t \times X_\theta| = a$. Thus a unit normal is

$$N = \frac{1}{a}(X_t \times X_\theta) = (-b' \cos \theta, -b' \sin \theta, a').$$

Second derivatives:

$$X_{tt} = (a'' \cos \theta, a'' \sin \theta, b''), \quad X_{t\theta} = (-a' \sin \theta, a' \cos \theta, 0),$$

$$X_{\theta\theta} = (-a \cos \theta, -a \sin \theta, 0).$$

Then

$$e := h(X_t, X_t) = \langle X_{tt}, N \rangle = -a''b' + a'b'',$$

$$f := h(X_t, X_\theta) = \langle X_{t\theta}, N \rangle = 0,$$

$$g := h(X_\theta, X_\theta) = \langle X_{\theta\theta}, N \rangle = ab'.$$

So, the matrices of the first and second fundamental forms in $\{X_t, X_\theta\}$ are

$$I = \begin{pmatrix} 1 & 0 \\ 0 & a^2 \end{pmatrix}, \quad II = \begin{pmatrix} -a''b' + a'b'' & 0 \\ 0 & ab' \end{pmatrix}.$$

The shape operator S satisfies $\Pi(v, w) = \langle Sv, w \rangle$. In matrix form, $S = \mathbf{I}^{-1}\Pi$, so

$$S = \begin{pmatrix} 1 & 0 \\ 0 & a^{-2} \end{pmatrix} \begin{pmatrix} -a''b' + a'b'' & 0 \\ 0 & ab' \end{pmatrix} = \begin{pmatrix} -a''b' + a'b'' & 0 \\ 0 & \frac{b'}{a} \end{pmatrix}.$$

Thus,

$$S(X_t) = k_1 X_t, \quad k_1(t) = -a''(t)b'(t) + a'(t)b''(t),$$

$$S(X_\theta) = k_2 X_\theta, \quad k_2(t) = \frac{b'(t)}{a(t)}.$$

So, X_t and X_θ are eigenvectors of S . Therefore, the direction tangent to the meridian is a principal direction; the direction tangent to the latitude circle is a principal direction.

(ii) For a surface in \mathbb{R}^3 , the Gaussian curvature is

$$K = \det S = k_1 k_2.$$

From above,

$$k_1 k_2 = (-a''b' + a'b'') \cdot \frac{b'}{a} = \frac{b'}{a} (a'b'' - b'a'').$$

Now use the unit-speed condition, we get

$$(a')^2 + (b')^2 = 1.$$

Differentiate it, we have

$$2a'a'' + 2b'b'' = 0 \implies a'a'' + b'b'' = 0 \implies b'b'' = -a'a''.$$

Then

$$(a'b'' - b'a'')b' = a'b''b' - b'^2a'' = a'(-a'a'') - b'^2a'' = -a'^2a'' - b'^2a'' = -(a'^2 + b'^2)a'' = -a''.$$

So

$$K = k_1 k_2 = \frac{(a'b'' - b'a'')b'}{a} = \frac{-a''}{a}.$$

Thus, the Gaussian curvature at $X(t, \theta)$ is

$$K(t, \theta) = -\frac{a''(t)}{a(t)}.$$

□

Problem 3

Proof. (i) Let a unit-speed curve like in problem 2 such that

$$\gamma(t) = (a(t), b(t)), \quad (a')^2 + (b')^2 = 1, \quad a(t) > 0,$$

revolved around the z -axis gives a surface of revolution

$$X(t, \theta) = (a(t) \cos \theta, a(t) \sin \theta, b(t)).$$

From Problem 2 we know

$$k_1(t) = -\frac{a''(t)}{b'(t)}, \quad k_2(t) = \frac{b'(t)}{a(t)}, \quad K(t, \theta) = k_1(t)k_2(t) = -\frac{a''(t)}{a(t)}.$$

To get $K \equiv 1$, we need

$$-\frac{a''(t)}{a(t)} = 1 \iff a''(t) + a(t) = 0.$$

For example, let

$$a(t) = 2 \cos t,$$

and restrict to the interval $I = (-\pi/6, \pi/6)$ so that $a(t) > 0$. Define b so that γ is unit speed as

$$(a')^2 + (b')^2 = 1 \implies 4 \sin^2 t + (b')^2 = 1 \implies b'(t) = \sqrt{1 - 4 \sin^2 t},$$

which is smooth and positive on I . Let

$$b(t) = \int_0^t \sqrt{1 - 4 \sin^2 s} \, ds.$$

Then $\gamma(t) = (a(t), b(t))$ is unit speed, $a > 0$, and the corresponding surface S is a surface of revolution. For this a we have $a''(t) = -2 \cos t = -a(t)$, so

$$K(t, \theta) = -\frac{a''(t)}{a(t)} = 1$$

for all $(t, \theta) \in I \times (0, 2\pi)$. Now look at one principal curvature

$$k_2(t) = \frac{b'(t)}{a(t)} = \frac{\sqrt{1 - 4 \sin^2 t}}{2 \cos t}.$$

At $t = 0$ we get

$$k_2(0) = \frac{1}{2}.$$

As $t \rightarrow \pi/6$, we have $\sin^2 t \rightarrow 1/4$, so $b'(t) \rightarrow 0$ while $\cos(\pi/6) = \sqrt{3}/2 \neq 0$, hence

$$\lim_{t \rightarrow \pi/6} k_2(t) = 0.$$

Thus, k_2 is not constant, so the principal curvatures of S are not constant, even though $K \equiv 1$.

(ii) For $w > 0$, consider

$$\gamma(t) = (a(t), b(t)) = (w \cosh(t/w), t), \quad t \in \mathbb{R},$$

and revolve it around the z -axis

$$X(t, \theta) = (a(t) \cos \theta, a(t) \sin \theta, b(t)).$$

Here, $a(t) = w \cosh(t/w)$, $b(t) = t$, so

$$a'(t) = \sinh(t/w), \quad a''(t) = \frac{1}{w} \cosh(t/w), \quad b'(t) = 1, \quad b''(t) = 0.$$

Computing first derivatives

$$X_t = (a' \cos \theta, a' \sin \theta, b'), \quad X_\theta = (-a \sin \theta, a \cos \theta, 0).$$

So, the first fundamental form is

$$\begin{aligned} E &= \langle X_t, X_t \rangle = a'^2 + b'^2 = \sinh^2(t/w) + 1 = \cosh^2(t/w), \\ F &= \langle X_t, X_\theta \rangle = 0, \quad G = \langle X_\theta, X_\theta \rangle = a^2 = w^2 \cosh^2(t/w). \end{aligned}$$

Then we have

$$X_t \times X_\theta = (-ab' \cos \theta, -ab' \sin \theta, aa') = (-a \cos \theta, -a \sin \theta, aa'),$$

so

$$|X_t \times X_\theta| = a\sqrt{E},$$

and a unit normal is

$$N = \frac{1}{a\sqrt{E}}(X_t \times X_\theta) = \frac{1}{\sqrt{E}}(-b' \cos \theta, -b' \sin \theta, a') = \frac{1}{\cosh(t/w)}(-\cos \theta, -\sin \theta, \sinh(t/w)).$$

Computing second derivatives

$$X_{tt} = (a'' \cos \theta, a'' \sin \theta, b''), \quad X_{t\theta} = (-a' \sin \theta, a' \cos \theta, 0), \quad X_{\theta\theta} = (-a \cos \theta, -a \sin \theta, 0).$$

Then the second fundamental form are

$$\begin{aligned} e &= \langle X_{tt}, N \rangle = \frac{-a''b' + a'b''}{\sqrt{E}} = \frac{-a''}{\sqrt{E}}, \\ f &= \langle X_{t\theta}, N \rangle = 0, \\ g &= \langle X_{\theta\theta}, N \rangle = \frac{ab'}{\sqrt{E}} = \frac{a}{\sqrt{E}}. \end{aligned}$$

Plug for a, a'', E :

$$E = \cosh^2(t/w), \quad \sqrt{E} = \cosh(t/w), \quad a = w \cosh(t/w), \quad a'' = \frac{1}{w} \cosh(t/w).$$

Hence,

$$\begin{aligned} e &= -\frac{a''}{\sqrt{E}} = -\frac{\frac{1}{w} \cosh(t/w)}{\cosh(t/w)} = -\frac{1}{w}, \\ g &= \frac{a}{\sqrt{E}} = \frac{w \cosh(t/w)}{\cosh(t/w)} = w. \end{aligned}$$

So e and g are constants. Since $F = f = 0$, the shape operator matrix in the basis $\{X_t, X_\theta\}$ is

$$S = \mathbf{I}^{-1}\mathbf{\Pi} = \begin{pmatrix} E^{-1} & 0 \\ 0 & G^{-1} \end{pmatrix} \begin{pmatrix} e & 0 \\ 0 & g \end{pmatrix} = \begin{pmatrix} \frac{e}{E} & 0 \\ 0 & \frac{g}{G} \end{pmatrix}.$$

Thus, the principal curvatures are

$$k_1 = \frac{e}{E} = \frac{-1/w}{\cosh^2(t/w)} = -\frac{1}{w \cosh^2(t/w)},$$

$$k_2 = \frac{g}{G} = \frac{w}{w^2 \cosh^2(t/w)} = \frac{1}{w \cosh^2(t/w)}.$$

Therefore,

$$k_1 + k_2 = 0,$$

so the mean curvature

$$H = \frac{k_1 + k_2}{2} = 0.$$

This implies M_w is a minimal surface for every $w > 0$. □

Problem 4

Proof. (i) Fix a point $p \in M$ and write $V = T_p M$ with inner product induced by g . For $w, x, y, z \in V$, define

$$B(w, x, y, z) := \langle w, y \rangle \langle x, z \rangle - \langle w, z \rangle \langle x, y \rangle.$$

For fixed y, z , this is alternating in (w, x) , and for fixed w, x it is alternating in (y, z) . By property of the exterior product in Lee's review, there exists a unique bilinear map

$$\langle \cdot, \cdot \rangle_{\Lambda^2} : \Lambda^2 V \times \Lambda^2 V \rightarrow \mathbb{R}$$

such that

$$\langle w \wedge x, y \wedge z \rangle_{\Lambda^2} = B(w, x, y, z) = \langle w, y \rangle \langle x, z \rangle - \langle w, z \rangle \langle x, y \rangle$$

for all $w, x, y, z \in V$.

We first check that $\langle \cdot, \cdot \rangle_{\Lambda^2}$ is an inner product. Let $\{e_1, \dots, e_n\}$ be an orthonormal basis of V . Then

$$\langle e_i \wedge e_j, e_k \wedge e_\ell \rangle_{\Lambda^2} = \delta_{ik} \delta_{j\ell} - \delta_{i\ell} \delta_{jk}.$$

In particular, for $i < j$ and $k < \ell$, this is 1 if $(i, j) = (k, \ell)$ and 0 otherwise. Thus, the family

$$\{e_i \wedge e_j : 1 \leq i < j \leq n\}$$

is an orthonormal basis of $\Lambda^2 V$, so $\langle \cdot, \cdot \rangle_{\Lambda^2}$ is symmetric and positive definite. Hence, it is an inner product on $\Lambda^2 V$. Then we compute the associated norm on decomposable 2-vectors

$$|w \wedge x|^2 = \langle w \wedge x, w \wedge x \rangle_{\Lambda^2} = \langle w, w \rangle \langle x, x \rangle - \langle w, x \rangle^2 = |w|^2 |x|^2 - \langle w, x \rangle^2.$$

This shows the existence.

For uniqueness, suppose $(\cdot, \cdot)'$ is any other fiber metric on $\Lambda^2 V$ whose associated norm satisfies

$$|w \wedge x|'^2 = |w|^2 |x|^2 - \langle w, x \rangle^2 \quad \text{for all } w, x \in V.$$

Let $\{e_1, \dots, e_n\}$ be an orthonormal basis of V . For $i < j$, we have

$$|e_i \wedge e_j|'^2 = |e_i|^2 |e_j|^2 - \langle e_i, e_j \rangle^2 = 1,$$

so each $e_i \wedge e_j$ has norm 1 with respect to $(\cdot, \cdot)'$. To see that they are orthogonal, fix distinct i, k and some j . Take $w = e_i + e_k$ and $x = e_j$. Then

$$w \wedge x = (e_i + e_k) \wedge e_j = e_i \wedge e_j + e_k \wedge e_j.$$

On one hand, by the given norm formula and orthonormality of e_i, e_j, e_k ,

$$|w \wedge x|^2 = |w|^2 |x|^2 - \langle w, x \rangle^2 = 2 \cdot 1 - 0 = 2.$$

On the other hand, expanding with the (unknown) inner product,

$$|w \wedge x|^2 = |e_i \wedge e_j + e_k \wedge e_j|^2 = |e_i \wedge e_j|^2 + |e_k \wedge e_j|^2 + 2(e_i \wedge e_j, e_k \wedge e_j)'.$$

Since each norm is 1, this is

$$2 = 1 + 1 + 2(e_i \wedge e_j, e_k \wedge e_j)' \implies (e_i \wedge e_j, e_k \wedge e_j)' = 0.$$

Similar choices of w, x show that $(e_i \wedge e_j, e_k \wedge e_\ell)' = 0$ whenever $(i, j) \neq (k, \ell)$ with $i < j, k < \ell$. Thus, $\{e_i \wedge e_j\}_{i < j}$ is an orthonormal basis for $(\cdot, \cdot)'$ as well. But on a finite-dimensional vector space, an inner product is uniquely determined by declaring a basis to be orthonormal. Hence, $(\cdot, \cdot)'$ coincides with $\langle \cdot, \cdot \rangle_{\Lambda^2}$. Therefore, the fiber metric constructed above is the unique one whose associated norm satisfies

$$|w \wedge x|^2 = |w|^2 |x|^2 - \langle w, x \rangle^2.$$

(ii) Fix $p \in M$ and write $V = T_p M$. Denote by Rm_p the curvature tensor at p :

$$\text{Rm}_p(w, x, y, z) = g_p(R(w, x)y, z).$$

Then it is multilinear and alternating in (w, x) and in (y, z) . Define first a bilinear form

$$B : \Lambda^2 V \times \Lambda^2 V \rightarrow \mathbb{R}$$

by

$$B(w \wedge x, y \wedge z) := -\text{Rm}_p(w, x, y, z),$$

and extend by bilinearity. This is well-defined by the universal property of $\Lambda^2 V$, because Rm_p is alternating in both (w, x) and (y, z) .

Now $(\Lambda^2 V, \langle \cdot, \cdot \rangle_{\Lambda^2})$ is a finite-dimensional inner product space. By linear algebra, any bilinear form B on such a space is represented by a unique linear operator $R_p : \Lambda^2 V \rightarrow \Lambda^2 V$ via

$$B(\alpha, \beta) = \langle R_p(\alpha), \beta \rangle_{\Lambda^2} \quad \text{for all } \alpha, \beta \in \Lambda^2 V.$$

Thus, there exists a unique linear map

$$R_p : \Lambda^2 T_p M \rightarrow \Lambda^2 T_p M$$

such that

$$\langle R_p(w \wedge x), y \wedge z \rangle_{\Lambda^2} = -\text{Rm}_p(w, x, y, z)$$

for all $w, x, y, z \in T_p M$.

These maps R_p vary smoothly with p . In a local orthonormal frame $\{E_i\}$ of TM , the frame $\{E_i \wedge E_j\}$ of $\Lambda^2(TM)$ is orthonormal, and we can write

$$R_p(E_i \wedge E_j) = \sum_{k < \ell} (-R_{ijkl}(p)) E_k \wedge E_\ell,$$

where R_{ijkl} are the components of the curvature tensor; these coefficients are smooth functions. Thus, R is a smooth bundle endomorphism

$$\mathcal{R} : \Lambda^2(TM) \rightarrow \Lambda^2(TM),$$

called the curvature operator of g , and it satisfies

$$\langle \mathcal{R}(w \wedge x), y \wedge z \rangle = -\text{Rm}(w, x, y, z)$$

for all tangent vectors w, x, y, z . Also, the uniqueness of \mathcal{R} follows from the fiberwise uniqueness of R_p . \square

Problem 5

Proof. Write

$$v(t) := \gamma'(t), \quad a(t) := D_t \gamma'(t)$$

for its velocity and covariant acceleration. Set

$$T(t) := \frac{v(t)}{|v(t)|},$$

the unit tangent field along γ . Choose an arc-length parameter s for γ , so that

$$\sigma(s) := \gamma(t(s)), \quad |\sigma'(s)| \equiv 1.$$

By def, the geodesic curvature of γ at t is

$$k(t) := |D_s T|_{s=s(t)},$$

where $T = \sigma'$ regarded as a unit tangent field along the unit-speed reparametrization. We express $D_s T$ in terms of t . Since

$$\frac{ds}{dt} = |v(t)|, \quad \frac{d}{ds} = \frac{1}{|v|} D_t,$$

we obtain

$$D_s T = \frac{1}{|v|} D_t T.$$

Now compute $D_t T$. Using $T = v/|v|$ and the product rule,

$$D_t T = D_t \left(\frac{v}{|v|} \right) = \frac{1}{|v|} a - \frac{1}{|v|^3} \langle a, v \rangle v.$$

Define the component of a orthogonal to v by

$$a_\perp := a - \frac{\langle a, v \rangle}{|v|^2} v.$$

Then

$$D_t T = \frac{1}{|v|} a_\perp, \quad D_s T = \frac{1}{|v|^2} a_\perp.$$

Hence

$$k(t) = |D_s T| = \frac{|a_\perp|}{|v|^2}.$$

By def of a_\perp ,

$$|a_\perp|^2 = |a|^2 - \frac{\langle a, v \rangle^2}{|v|^2}.$$

On the other hand, by Problem 4,

$$|v \wedge a|^2 = |v|^2 |a|^2 - \langle v, a \rangle^2.$$

Combining these,

$$|a_\perp|^2 = \frac{|v \wedge a|^2}{|v|^2}.$$

Therefore,

$$k(t)^2 = \frac{|a_\perp|^2}{|v|^4} = \frac{|v \wedge a|^2}{|v|^6},$$

and taking square roots gives

$$k(t) = \frac{|\gamma'(t) \wedge D_t \gamma'(t)|}{|\gamma'(t)|^3}.$$

Here the norm in the numerator is the one induced on $\Lambda^2(TM)$ as in Problem 4. Now assume $M = \mathbb{R}^3$ with the Euclidean metric. There is a natural identification between 2-vectors and vectors via the cross product. For $u, v \in \mathbb{R}^3$, $u \times v$ corresponds to $u \wedge v \in \Lambda^2 \mathbb{R}^3$, and this identification is an isometry, so

$$|u \times v| = |u \wedge v|.$$

Thus, for $\gamma : I \rightarrow \mathbb{R}^3$,

$$k(t) = \frac{|\gamma'(t) \wedge \gamma''(t)|}{|\gamma'(t)|^3} = \frac{|\gamma'(t) \times \gamma''(t)|}{|\gamma'(t)|^3}.$$

□

Problem 6

Proof. Fix $p \in M$ and write $V = T_p M \subset \mathbb{R}^{n+1}$. For any $X \in V$, consider N as a vector field along M in \mathbb{R}^{n+1} . Then

$$d\nu_p(X) = D_X N \in T_{\nu(p)} S^n \subset \mathbb{R}^{n+1},$$

where D is the ordinary derivative in \mathbb{R}^{n+1} .

Because $|N|^2 \equiv 1$, we have

$$0 = X(\langle N, N \rangle) = 2\langle D_X N, N \rangle,$$

so $D_X N \perp N$. Since both $T_p M$ and $T_{\nu(p)} S^n$ are the hyperplane $\{v \in \mathbb{R}^{n+1} : \langle v, N_p \rangle = 0\}$, we have $D_X N \in T_p M$ and $D_X N \in T_{\nu(p)} S^n$ simultaneously.

By definition of the shape operator S of M (Lee, §8.2),

$$S_p(X) = -D_X N \in T_p M.$$

Thus, viewing $T_p M$ and $T_{\nu(p)} S^n$ as the same subspace of \mathbb{R}^{n+1} ,

$$d\nu_p = -S_p : T_p M \rightarrow T_{\nu(p)} S^n.$$

Both $T_p M$ and $T_{\nu(p)} S^n$ are n -dimensional oriented inner product spaces, with volume forms $(dV_g)_p$ and $(dV_{g_0})_{\nu(p)}$. Let e_1, \dots, e_n be an oriented orthonormal basis of $T_p M$. Since N_p is the outward unit normal for both M and S^n , we may regard e_1, \dots, e_n also as an oriented orthonormal basis of $T_{\nu(p)} S^n$ (the condition that (N_p, e_1, \dots, e_n) is an oriented orthonormal basis of \mathbb{R}^{n+1} is the same in both cases).

By definition of the pullback of a top-degree form,

$$(\nu^* dV_{g_0})_p(e_1, \dots, e_n) = (dV_{g_0})_{\nu(p)}(d\nu_p(e_1), \dots, d\nu_p(e_n)).$$

In an oriented orthonormal basis, a volume form is just the determinant:

$$(dV_{g_0})_{\nu(p)}(d\nu_p(e_1), \dots, d\nu_p(e_n)) = \det(d\nu_p) (dV_{g_0})_{\nu(p)}(e_1, \dots, e_n).$$

But $(dV_{g_0})_{\nu(p)}(e_1, \dots, e_n) = 1$ and $(dV_g)_p(e_1, \dots, e_n) = 1$, so

$$(\nu^* dV_{g_0})_p(e_1, \dots, e_n) = \det(d\nu_p) = \det(-S_p).$$

If $\kappa_1, \dots, \kappa_n$ are the principal curvatures of M at p , then S_p is diagonalizable in an orthonormal basis with eigenvalues $\kappa_1, \dots, \kappa_n$, so

$$\det(S_p) = \kappa_1 \cdots \kappa_n =: K(p)$$

is the Gaussian curvature of M at p (product of principal curvatures). Hence

$$\det(d\nu_p) = \det(-S_p) = (-1)^n \det(S_p) = (-1)^n K(p).$$

Therefore,

$$(\nu^* dV_{g_0})_p(e_1, \dots, e_n) = (-1)^n K(p) = ((-1)^n K dV_g)_p(e_1, \dots, e_n).$$

Since this holds for all oriented orthonormal bases of $T_p M$, we conclude

$$\nu^* dV_{g_0} = (-1)^n K dV_g.$$

□